@@ -1,7 +1,6 @@
 From STLC Require Import STLC_SuccNat.
 Require Export STLC_SuccNat.
 
-
 Fixpoint cstep (t:tm) : tm :=
   match t with
   | var x => var x
@@ -18,13 +17,13 @@ Fixpoint cstep (t:tm) : tm :=
 Compute cstep (succ (succ (const 1))).
 
 Fixpoint mcstep (i:nat) (t:tm) : option tm :=
-  match cstep t with
+  match t with
   | var x => Some (var x)
   | abs x T t => Some (abs x T t)
   | const n => Some (const n)
-  | t1 => match i with
+  | t => match i with
           | O => None
-          | S i' => mcstep i' t1
+          | S i' => mcstep i' (cstep t)
     end
   end.
 
@@ -35,6 +34,7 @@ Compute cstep (cstep (app (abs "x" Nat (succ (var "x"))) (const 4))).
 Compute mcstep 2 (app (abs "x" Nat (succ (var "x"))) (const 4)).
 
 Compute mcstep 0 (var "x").
+Compute mcstep 0 (succ (const 1)).
 
 Lemma step__cstep: forall t1 t2,
   step t1 t2 -> cstep t1 = t2.
@@ -77,7 +77,7 @@ Proof.
   (* fixp *)
   - remember (cstep t1) as t2_1.
     simpl in H. destruct t1;
-    try ( apply IHt1 in Heqt2_1 as [];
+    try (apply IHt1 in Heqt2_1 as [];
       try solve_by_inverts 2; [
         (left; rewrite <- H;
           apply ST_Fixp; assumption)|
@@ -90,7 +90,7 @@ Proof.
   (* succ *)
   - remember (cstep t1) as t2_1.
     simpl in H. destruct t1;
-    try ( apply IHt1 in Heqt2_1 as [];
+    try (apply IHt1 in Heqt2_1 as [];
       try solve_by_inverts 2; [
         (left; rewrite <- H;
           apply ST_Succ; assumption)|
@@ -103,33 +103,37 @@ Qed.
 Lemma mcstep_nf: forall i t v,
   mcstep i t = Some v -> normal_form step v.
 Proof.
-  induction i; intros; 
-    destruct (cstep t) eqn:Eq;
-      (simpl in H; rewrite Eq in H);
-      try discriminate;
-      try (injection H as H; subst;
+  induction i; intros;
+    destruct t eqn:Eqt;
+    try discriminate; 
+    try (injection H as H; subst;
             intros [x contra]; inversion contra);
-    eapply IHi; eassumption.
+    try (destruct (cstep t) eqn:Eq;
+         (subst; simpl in *; rewrite Eq in H;
+          eapply IHi; eassumption)).
 Qed.
 
 Lemma msctep__mstep: forall i t v,
   mcstep i t = Some v -> multi step t v.
 Proof.
   induction i; intros;
-    destruct (cstep t) eqn:Eq;
-    (simpl in H; rewrite Eq in H);
+    destruct t eqn:Eqt;
     try discriminate;
-    try (
-      injection H as H; subst;
-      apply cstep__step in Eq;
-      destruct Eq; [
-        eapply multi_step; [eassumption|] |
-        subst]; apply multi_refl
-    );
+    try (injection H as H; subst; apply multi_refl);
+    try (unfold mcstep in H;
+    destruct (cstep t) eqn:Eq; subst;
+    rewrite Eq in H; fold mcstep in H;
     try (apply cstep__step in Eq;
-        destruct Eq; [
-        eapply multi_step; [| apply IHi]; eassumption |
-        subst; apply IHi; assumption ]).
+         destruct Eq; [
+          eapply multi_step; [|apply IHi]; eassumption |
+          discriminate
+         ]);
+    apply cstep__step in Eq;
+    destruct Eq; [
+    eapply multi_step; [eassumption|];
+    apply IHi; assumption |
+    injection H0 as H0; subst;
+    apply IHi; assumption ]).
 Qed.
 
 Corollary mcstep__snf: forall i t v,
@@ -151,12 +155,76 @@ Proof.
   eassumption.
   eapply mcstep__snf.
   eassumption.
-Qed.  
+Qed.
 
-Theorem snf__mcstep: forall t v,
+Lemma mcstep_succ: forall i t n,
+  mcstep i t = Some (const n) ->
+  mcstep (S i) (succ t) = Some (const (S n)).
+Proof.
+  intros. unfold mcstep.
+  destruct (cstep (succ t)) eqn:Eq;
+  rewrite <- Eq; fold mcstep;
+  try (simpl; destruct (match t with
+            | const n0 => const (S n0)
+            | _ => succ (cstep t)
+            end) eqn:Eqt;
+      try (destruct t; discriminate)).
+  - destruct i; destruct t;
+    try discriminate;
+      (simpl in H; injection H as H;
+      injection Eqt as Eqt;
+      subst; reflexivity).
+  - induction i; destruct t;
+    try discriminate.
+    + injection Eq as Eq.
+      simpl in H. rewrite Eq in H.
+      simpl in Eqt. rewrite Eq in Eqt.
+      rewrite <- Eqt. simpl.
+Abort.
+
+Theorem snf__mcstep: forall t v T,
+  has_type empty t T ->
   step_normal_form_of t v ->
   exists i,  mcstep i t = Some v.
 Proof.
+  intros t v T HT [Hms Hnf].
+  generalize dependent T.
+  generalize dependent v.
+  induction t; intros.
+  (* var *)
+  - solve_by_inverts 2.
+  (* app *)
+  - pose proof (app_fun_normalizes_first _ _ _ _ HT (conj Hms Hnf)) as
+    [x [T1 [u Ht1]]]. 
+    inversion HT; subst.
+    clear IHt2 H4.
+    assert (normal_form step (abs x T1 u)).
+    { intros [x0 contra]; inversion contra. }
+    pose proof (IHt1 _ Ht1 H _ H2) as [i H0].
+    clear H H2 Ht1 T2. admit.
+  (* abs *)
+  - inversion Hms; subst.
+  exists 0; auto.
+  solve_by_inverts 1.
+  (* fixp *)
+  - admit.
+  (* const *)
+  - inversion Hms; subst.
+    exists 0; auto.
+    solve_by_inverts 1.
+  (* succ *)
+  - pose proof (succ_arg_normalizes_first _ _ _ HT (conj Hms Hnf))
+    as [n H].
+    assert (normal_form step (const n)) by (intros []; solve_by_inverts 1).
+    inversion HT; subst.
+    pose proof (IHt (const n) H H0 Nat H3) as [i H1].
+    exists (S i). clear IHt.
+    destruct t eqn:Eq;
+    try solve_by_inverts 2.
+    + unfold mcstep. 
+
+
+
   induction t; intros.
   (* var *)
   - inversion H;
@@ -164,5 +232,6 @@ Proof.
     exists 1; auto.
     inversion H2.
   (* app *)
-  - inversion H.
+  - 
+
 Abort.
